\section{Question 3}

\textbf{3a)} The conditional distribution of Y can be expressed as:
$$P(Y = y | X = x)  = \frac{f_{xy}(x,y)}{f_{x}(X = X)}$$

\begin{equation}
    \begin{split}
        P(Y = y | X = x)  = \frac{f_{xy}(x,y)}{f_{x}(X = X)} = Exp(x) \\ \\
        \text{Given P(X = x) = Exp(1)} \\ \\
        P(Y = y | X = x)  = \frac{f_{xy}}{Exp(1)} = Exp(x) \\ \\
        f_{xy}(X, Y) = Exp(x)Exp(1) = e^{-x} \left(xe^{-yx}\right)\\ \\
        \text{Now that we have Fxy(X, Y), we can find the marginal distribution of Y by } F_y(y) = \int^{\infty}_{-\infty} fxy(x,y,) dx \\\\
        f_y(y) = \int^{\infty}_{-\infty} fxy(x,y,) dx \\
        = \int^{\infty}_{-\infty} e^{-x} \left(xe^{-yx}\right) dx \\
        \text{Because -infinity approaches 0, we can change the bounds to that} \\
        = \int^{\infty}_{0} e^{-x} \left(xe^{-yx}\right) dx \\
        = \int e^{-yx-x}xdx \\
        u=x, v'=e^{-yx-x} \\
        = e^{-yx-x}\frac{1}{-y-1}x-\int e^{-yx-x}\frac{1}{-y-1}dx \\
        = e^{-yx-x}\frac{1}{-y-1}x-e^{-yx-x}\frac{1}{\left(-y-1\right)^2} \\
        = \left[e^{-yx-x}\frac{1}{-y-1}x-e^{-yx-x}\frac{1}{\left(-y-1\right)^2}\right]^\infty_0 \\
        = 0 - \left(-\frac{1}{\left(-y-1\right)^2}\right) \\
        F_y(Y) = \frac{1}{\left(-y-1\right)^2}  \\
        \implies \text{The marginal probability density function of Y} = \frac{1}{\left(-y-1\right)^2}
    \end{split}
\end{equation}

\textbf{3b)} Now that we have the marginal pdf of Y, we can calculate $E[X | Y = y]$: \\
$$P(X = x | Y = y)  = \frac{f_{xy}(x,y)}{f_{y}(Y = y)}$$

\begin{equation}
    \begin{split}
        P(X = x | Y = y)  = \frac{f_{xy}(x,y)}{f_{y}(Y = y)}\\
        = \frac{e^{-x} \left(xe^{-yx}\right)}{\frac{1}{\left(-y-1\right)^2}} \\
        = e^{-x-xy}x\left(-y-1\right)^2 \\
        \implies E[X | Y = y] = e^{-x-xy}x\left(-y-1\right)^2
    \end{split}
\end{equation}





\end{document}